dafny/boolean_algebra/syntax.dfy
@@ -7,25 +7,27 @@ module expression
 
     /*
     We use the definition of the syntax of Boolean expressions
-    to introduce the fundamental concept of inductive definitions.
-    Inductive definitions of data types representing often infinite 
-    sets of values is done by first defining a set starting values
-    (like base cases for a recursion) and then by defining rules for 
-    forming new values from ones already defined. 
+    to introduce the fundamental concept of inductive 
+    definitions. Inductive definitions of data types 
+    representing often infinite sets of values is done by 
+    first defining a set starting values (like base cases for 
+    a recursion) and then by defining rules for forming new 
+    values from ones already defined. 
     */
 
 
     /*
-    Here the base values are the terms litTrue and litFalse. We 
-    will eventually interpret them as "literal" terms representing
-    the Boolean values, true and false.
+    Here the base values are the terms litTrue and litFalse. 
+    We will eventually interpret them as "literal" terms 
+    representing the Boolean values, true and false.
     */
     datatype bExp = 
         bTrue |
         bFalse | 
         bNot (e: bExp) |
         bAnd (e1: bExp, e2: bExp) |
-        bOr (e1: bExp, e2: bExp)
+        bOr (e1: bExp, e2: bExp) | 
+        bImpl (e1: bExp, e2: bExp)
 
 
     /*
@@ -36,26 +38,32 @@ module expression
     that were passed to the constructor, and then recursively 
     printing subparts until the base cases are reached.
     */
-
     function method show_bExp(e: bExp): string
     {
         match e 
         {
             case bTrue => "True"
             case bFalse => "False"
-            case bNot (e: bExp) => 
-                "NOT (" + show_bExp(e) + ")"
+            case bNot (e': bExp) => 
+                "NOT (" + show_bExp(e') + ")"
             case bAnd (e1: bExp, e2: bExp) => 
                 "AND (" + show_bExp(e1) + ", " + show_bExp(e2) + ")"
             case bOr (e1: bExp, e2: bExp) =>  
                 "OR (" + show_bExp(e1) + ", " + show_bExp(e2) + ")"
-            
+            case bImpl (e1: bExp, e2: bExp) =>  
+                "-> (" + show_bExp(e1) + ", " + show_bExp(e2) + ")"   
         }
     }
 
-       function method show_bExp_infix(e: bExp): string
+    /*
+    This function returns a string representing the given
+    Boolean expression using prefix notation. It inserts
+    parenthesis "with abandon" to disambiguate the order
+    of operations in complex expressions.
+    */
+    function method show_bExp_infix(e: bExp): string
     {
-        match e 
+    match e 
         {
             case bTrue => "True"
             case bFalse => "False"
@@ -65,8 +73,8 @@ module expression
                 "(" + show_bExp_infix(e1) + " AND " + show_bExp_infix(e2) + ")"
             case bOr (e1: bExp, e2: bExp) =>  
                 "(" + show_bExp_infix(e1) + " OR " + show_bExp_infix(e2) + ")"
-            
+            case bImpl (e1: bExp, e2: bExp) =>  
+                "(" + show_bExp_infix(e1) + " -> " + show_bExp_infix(e2) + ")"        
         }
     }
-
 }
