dafny/predicate-logic/interpretation.dfy
@@ -14,36 +14,38 @@
     we'll  look up the value of the variable in such
     a map. 
 
-    We define a "type synonym," pInterpretation, for 
-    map<bVar,bool>. Type synonyms don't change the 
+    We define a "type synonym," pInterpretation, short
+    for "propositional logic interpretation", for the
+    map<bVar,bool> type. Type synonyms don't change the 
     behavior of code. Rather, they serve to document 
     the purpose of the code for human readers. In this 
     sense, they support a form of "abstraction", hiding 
     complex details behind a simpler, meaningful name.
+    pInterpreation means exactly map<propVar, bool>.
     */
-
     type pInterpretation = map<propVar, bool>
 
  
     /*
     This method returns the value assigned to a given
-    propositional variable by a given interpretation,
-    or false if the variable's not mapped by it. The
-    design of this code would be improved by the
-    addition of a precondition that requires v in i.
+    propositional variable by a given interpretation.
+    This function can only be called with a variable, v,
+    for which the given interpretation, i, has a value.
+    However, this pre-condition is not formalized or
+    enforced.
     */
     function method pVarValue(v: propVar, i: pInterpretation): bool
+        requires v in i
     {
-        if (v in i) then i[v] else false
+        i[v]
     }
 
     /*
     This method serializes an interpretation to a string,
     using the string name of each variable in the output.
-    The design would be improved by a pre-condition that
-    requires forall v :: v in vs ==> v in interp.
     */
     method show_interpretation (interp: pInterpretation, vs: seq<propVar>,labels: bool)
+    //    requires forall v :: v in vs ==> v in interp
     {
         var n := | vs |;
         var i := 0;
@@ -66,17 +68,19 @@
  is mainly used to output, for example, lists of models 
  or counterexamples of given propositions.
  */
- method show_interpretations(interps: seq<pInterpretation>, vs: seq<propVar>, labels: bool)
-    {
-        var i := 0;
-        print "{\n";
-        while (i < |interps|)
+method show_interpretations(interps: seq<pInterpretation>, vs: seq<propVar>, labels: bool)
+    //requires forall i :: 0 <= i < |interps| ==> 
+    //    (forall v :: v in vs ==> v in interps[i])
+{
+    var i := 0;
+    print "{\n";
+    while (i < |interps|)
         {
             show_interpretation(interps[i], vs, labels);
             if i < |interps| - 1 { print ",\n"; }
             i := i + 1;
         }
-        print "\n}\n";
+     print "\n}\n";
     }
  }
 
